{
 "cells": [
  {
   "cell_type": "markdown",
   "metadata": {},
   "source": [
    "# Name: Nica Samantha A. Antiporta\n",
    "# Course: BSCS-1\n",
    "# Id: 22102103\n",
    "# Questions:\n",
    "---\n",
    "\n",
    "### Why is Proof Necessary?\n",
    "\n",
    "Proofs play a vital role in confirming whether a statement or theorem is true. They provide logical reasoning that demonstrates the validity of a claim, ensuring its reliability under specific circumstances. This reliability enables us to use the statement confidently in various calculations, deductions, or practical applications.\n",
    "\n",
    "    \n",
    "### Consequences of Failing to Provide a Proof\n",
    "\n",
    "Without a proof, we can't be sure if a statement or theorem is true. This uncertainty makes it hard to know if the claim applies in different situations. So, the statement stays uncertain, making it tough to use in solving problems or understanding things better."
   ]
  },
  {
   "cell_type": "markdown",
   "metadata": {},
   "source": [
    "Problem no. 1 Prove that the Euler's number $e = \\Sigma_{k=0}^\\infty \\frac{1}{k!} \\notin \\mathbb{Q}$.\n",
    "---\n",
    "Recall that a rational number is one that can be expressed as the quotient of two integers. We want to prove that Euler's number $e = \\sum_{k=0}^\\infty \\frac{1}{k!} \\notin \\mathbb{Q}$.\n",
    "\n",
    "**Proof by Contradiction**\n",
    "\n",
    "We will assume the opposite (that `e` is rational) and show that this leads to a contradiction.\n",
    "\n",
    "* **Definition of Rational Numbers:**\n",
    "\n",
    "A rational number is any number that can be expressed as a quotient (`a / b`), where `a` and `b` are integers, and `b ≠ 0`.\n",
    "\n",
    "* **Assume e is Rational:**\n",
    "\n",
    "For the sake of contradiction, let's assume `e` can be expressed as a fraction `a / b`, where `a` and `b` are integers.\n",
    "\n",
    "* **Series Expansion of e:**\n",
    "\n",
    "We know the series expansion of `e`:\n",
    "\n",
    "$$ e = \\sum_{k=0}^\\infty \\frac{1}{k!} = 1 + \\frac{1}{1!} + \\frac{1}{2!} + \\frac{1}{3!} + \\dotsb $$\n",
    "\n",
    "* **Multiplying by b!**\n",
    "\n",
    "Let's multiply both sides of the equation by `b!` to eliminate the factorials:\n",
    "\n",
    "$$ b!e = b! \\left(1 + \\frac{1}{1!} + \\frac{1}{2!} + \\frac{1}{3!} + \\dotsb \\right) = b! (1 + b + \\frac{b(b-1)}{2!} + \\frac{b(b-1)(b-2)}{3!} + \\dotsb) $$\n",
    "\n",
    "* **Contradiction:**\n",
    "\n",
    "Observe that every term on the right side of the equation is now a multiple of `b!` because it includes `b!` or a product of factors containing `b`. Since the product of integers is an integer, the entire right side becomes an integer. This contradicts our initial assumption that `e = a / b` (where `b` is an integer). \n",
    "\n",
    "Therefore, our assumption that `e` is rational must be false. \n",
    "\n",
    "**Conclusion:**\n",
    "\n",
    "By contradiction, we have proven that Euler's number `e` is irrational (i.e., it cannot be expressed as a fraction of two integers).\n",
    "\n",
    "Observe that since each term on the right side of the equation is a multiple of $b!$, the entire expression is an integer. Consequently, if $e$ were rational, it would contradict our initial assumption. Thus, $e \\notin \\mathbb{Q}$."
   ]
  },
  {
   "cell_type": "markdown",
   "metadata": {},
   "source": [
    "Problem no. 2 \n",
    "Prove Minkowski's Inequality for sums, $\\forall \\ p>1, (a_k, b_k)>0$:\n",
    "---\n",
    "\n",
    "We want to prove Minkowski's Inequality for sums and thus:\n",
    "\\[ $\\left(\\sum_{k=1}^n |a_k + b_k|^p\\right)^\\frac{1}{p} \\leq \\left(\\sum_{k=1}^n |a_k|^p\\right)^\\frac{1}{p} + \\left(\\sum_{k=1}^n |b_k|^p\\right)^\\frac{1}{p} $\\]\n",
    "\n",
    "$\\textit{Proof:}$\n",
    "\n",
    "The proof involves utilizing Hölder's inequality. Let \\( q \\) be the conjugate exponent of \\( p \\). (i.e., $\\frac{1}{p} + \\frac{1}{q} = 1$).\n",
    "\n",
    "Apply Hölder's inequality with $p$ and $q$ to the sequences $(|a_k|^p)$ and $(1)$, and to the sequences $(|b_k|^p)$ and $(1)$:\n",
    "\n",
    "\\[ $\\sum_{k=1}^n |a_k|^p \\cdot 1 \\leq \\left(\\sum_{k=1}^n |a_k|^p\\right)^\\frac{1}{p} \\left(\\sum_{k=1}^n 1^q\\right)^\\frac{1}{q} = \\left(\\sum_{k=1}^n |a_k|^p\\right)^\\frac{1}{p} \\cdot n^\\frac{1}{q} $\\]\n",
    "\n",
    "then.\n",
    "\n",
    "\\[ $\\sum_{k=1}^n |b_k|^p \\cdot 1 \\leq \\left(\\sum_{k=1}^n |b_k|^p\\right)^\\frac{1}{p} \\left(\\sum_{k=1}^n 1^q\\right)^\\frac{1}{q} = \\left(\\sum_{k=1}^n |b_k|^p\\right)^\\frac{1}{p} \\cdot n^\\frac{1}{q} $\\]\n",
    "\n",
    "Add these inequalities:\n",
    "\n",
    "\\[ $\\sum_{k=1}^n |a_k|^p + \\sum_{k=1}^n |b_k|^p \\leq \\left(\\sum_{k=1}^n |a_k|^p\\right)^\\frac{1}{p} \\cdot n^\\frac{1}{q} + \\left(\\sum_{k=1}^n |b_k|^p\\right)^\\frac{1}{p} \\cdot n^\\frac{1}{q} $\\]\n",
    "\n",
    "then.\n",
    "\n",
    "\\[ $\\sum_{k=1}^n (|a_k|^p + |b_k|^p) \\leq \\left(\\sum_{k=1}^n |a_k|^p\\right)^\\frac{1}{p} \\cdot n^\\frac{1}{q} + \\left(\\sum_{k=1}^n |b_k|^p\\right)^\\frac{1}{p} \\cdot n^\\frac{1}{q} $\\]\n",
    "\n",
    "After this we raise both sides to the power of $\\frac{1}{p}$:\n",
    "\n",
    "\\[ $\\left(\\sum_{k=1}^n (|a_k|^p + |b_k|^p)\\right)^\\frac{1}{p} \\leq \\left(\\left(\\sum_{k=1}^n |a_k|^p\\right)^\\frac{1}{p} \\cdot n^\\frac{1}{q} + \\left(\\sum_{k=1}^n |b_k|^p\\right)^\\frac{1}{p} \\cdot n^\\frac{1}{q}\\right)^\\frac{1}{p} $\\]\n",
    "\n",
    "then.\n",
    "\n",
    "\\[ $\\left(\\sum_{k=1}^n (|a_k + b_k|^p)\\right)^\\frac{1}{p} \\leq \\left(\\sum_{k=1}^n |a_k|^p\\right)^\\frac{1}{p} + \\left(\\sum_{k=1}^n |b_k|^p\\right)^\\frac{1}{p} $\\]\n",
    "\n",
    "Thus this then proves Minkowski's Inequality."
   ]
  },
  {
   "cell_type": "markdown",
   "metadata": {},
   "source": [
    "Problem no. 3 Prove the triangle inequality $|x+y| \\leq |x| + |y|, \\forall (x,y) \\in \\mathbb{R}$\n",
    "---\n",
    "\n",
    "$\\textit{Proof:}$\n",
    "\n",
    "Consider these three cases:\n",
    "\n",
    "1. If $x \\geq 0$ and $y \\geq 0$, then $|x| = x$ and $|y| = y$, so $|x+y| = x+y$. Then $|x+y| = x + y \\leq |x| + |y|$.\n",
    "   \n",
    "3. If $x \\geq 0$ and $y < 0$, then $|x| = x$ and $|y| = -y$, so $|x+y| = x-y$. Then $|x+y| = x - y \\leq |x| + |y|$.\n",
    "   \n",
    "4. If $x < 0$ and $y < 0$, then $|x| = \n",
    "-x$ and $|y| = -y$, so $|x+y| = -(x+y) = -x - y$. Then $|x+y| = -(x + y) \\leq |x| + |y|$."
   ]
  },
  {
   "cell_type": "markdown",
   "metadata": {},
   "source": [
    "## Problem 4: Prove Sedrakayan's Lemma\n",
    "\n",
    "**Lemma:** $\\forall u_i, v_i \\in \\mathbb{R}^+$:\n",
    "\n",
    "$\\frac{(\\sum_{i=1}^n u_i)^2}{\\sum_{i=1}^n v_i} \\leq \\sum_{i=1}^n \\frac{(u_i)^2}{v_i}$\n",
    "\n",
    "**Proof:**\n",
    "\n",
    "1. **Define vectors:** Let $\\mathbf{u} = (u_1, u_2, ..., u_n)$ and $\\mathbf{v} = (v_1, v_2, ..., v_n)$ be vectors in $\\mathbb{R}^+$.\n",
    "\n",
    "2. **Cauchy-Schwarz Inequality:** Apply Cauchy-Schwarz Inequality:\n",
    "\n",
    "$(\\sum_{i=1}^n u_i v_i)^2 \\leq (\\sum_{i=1}^n u_i^2) (\\sum_{i=1}^n v_i^2)$\n",
    "\n",
    "3. **Divide by norm:** Since $v_i > 0$ for all $i$, divide both sides by $\\sum_{i=1}^n v_i^2$:\n",
    "\n",
    "$\\frac{(\\sum_{i=1}^n u_i v_i)^2}{(\\sum_{i=1}^n v_i^2)} \\leq \\sum_{i=1}^n u_i^2$\n",
    "\n",
    "4. **Vector notation:** Introduce vector dot product $(\\mathbf{u} \\cdot \\mathbf{v})$ and Euclidean norm $\\|\\cdot\\|$:\n",
    "\n",
    "$\\frac{(\\mathbf{u} \\cdot \\mathbf{v})^2}{\\|\\mathbf{v}\\|^2} \\leq \\|\\mathbf{u}\\|^2$\n",
    "\n",
    "5. **Square both sides:**\n",
    "\n",
    "$\\frac{(\\mathbf{u} \\cdot \\mathbf{v})^2}{\\|\\mathbf{v}\\|^4} \\leq \\frac{\\|\\mathbf{u}\\|^2}{\\|\\mathbf{v}\\|^2}$\n",
    "\n",
    "6. **Substitute and rearrange:** Substitute $\\|\\mathbf{v}\\|^2 = \\sum_{i=1}^n v_i$ and rearrange:\n",
    "\n",
    "## $\\frac{(\\sum_{i=1}^n u_i)^2}{\\sum_{i=1}^n v_i} \\leq \\sum_{i=1}^n \\frac{u_i^2}{v_i}$\n",
    "\n",
    "\n"
   ]
  },
  {
   "cell_type": "markdown",
   "metadata": {},
   "source": [
    "## Problem 5\n",
    "\n",
    "Consider the functions $ f(x) = 2x + 1 , ( g(x) = 2y - 1 ), ( j(x) = |f(x) + g(x)| ), and ( h(x) = j(x)^2 )$. Show that the following inequality holds:\n",
    "\n",
    "$\\sqrt{|f(x)|^2} \\geq \\sqrt{h(x)} - \\sqrt{|g(x)|^2}, \\quad \\forall (x, y) \\in \\mathbb{Z}^+\n",
    "$\n",
    "\n",
    "Thus then we substitute the functions:\n",
    "\n",
    "$\n",
    "\\sqrt{(2x+1)^{2}} \\geq \\sqrt{|(2x + 1) + (2y - 1)|^{2}} - \\sqrt{(2y-1)^{2}}\n",
    "$\n",
    "\n",
    "Given the properties of absolute value, we understand that certain mathematical principles and inequalities are valid.\n",
    "\n",
    "$\n",
    "\\sqrt{(x)^{2}} = |x|\n",
    "$\n",
    "\n",
    "Thus we get this: \n",
    "\n",
    "$\n",
    "|2x + 1| \\geq |(2x + 1) + (2y - 1)| - |2y - 1|\n",
    "$"
   ]
  },
  {
   "cell_type": "markdown",
   "metadata": {},
   "source": [
    "Let's simplify the expression by assigning variables to the terms:\n",
    "\n",
    "Let $a = 2x + 1$ and $b = 2y - 1$\n",
    "\n",
    "$\n",
    "|a| \\geq |a + b| - |b|\n",
    "$\n",
    "\n",
    "By adding $|b|$ to both sides and subtracting $|a|$, we arrive at:\n",
    "\n",
    "$\n",
    "|a + b| \\leq |a| + |b|\n",
    "$\n",
    "\n",
    "\n",
    "The provided inequality simply represents the triangle inequality theorem."
   ]
  },
  {
   "cell_type": "markdown",
   "metadata": {},
   "source": [
    "## PROBLEM 6: Sedrakayan's Lemma  2\n",
    "\n",
    "Demonstrate Sedrakayan's Lemma when $u_i$ and $v_i$ are square roots of an even integer, where $u_i = 2a_i$ and $v_i = 2b_i$, with $a_i, b_i$ being integers.\n",
    "\n",
    "## $\\frac{(\\sum_{i=1}^{n}2a_i)^{2}}{\\sum_{i=1}^{n}2b_i} \\leq \\sum_{i=1}^{n} \\frac{(2a_i)^{2}}{2b_i}$\n",
    "\n",
    "then simplified to:\n",
    "\n",
    "## $ \\frac{4(\\sum_{i=1}^{n}a_i)^{2}}{2\\sum_{i=1}^{n}b_i} \\leq \\sum_{i=1}^{n} \\frac{4(a_i)^{2}}{2b_i}$\n",
    "\n",
    "then simplified to:\n",
    "\n",
    "## $\\frac{2(\\sum_{i=1}^{n}a_i)^{2}}{\\sum_{i=1}^{n}b_i} \\leq 2\\space[\\sum_{i=1}^{n} \\frac{(a_i)^{2}}{b_i}]$\n",
    "\n",
    "both sides need to be multiplied by $\\frac{1}{2}$\n",
    "\n",
    "## $\\frac{(\\sum_{i=1}^{n}a_i)^{2}}{\\sum_{i = 1}^{n}b_i} \\leq \\sum_{i=i}^{n} \\frac{(a_i)^{2}}{b_i}$\n",
    "\n",
    "\n",
    "In conclusion, Sedrakayan's Lemma states that for square roots of an even integer, represented by \n",
    "are integers. This holds true.\n"
   ]
  },
  {
   "cell_type": "code",
   "execution_count": null,
   "metadata": {},
   "outputs": [],
   "source": []
  }
 ],
 "metadata": {
  "kernelspec": {
   "display_name": "Python 3 (ipykernel)",
   "language": "python",
   "name": "python3"
  },
  "language_info": {
   "codemirror_mode": {
    "name": "ipython",
    "version": 3
   },
   "file_extension": ".py",
   "mimetype": "text/x-python",
   "name": "python",
   "nbconvert_exporter": "python",
   "pygments_lexer": "ipython3",
   "version": "3.12.2"
  }
 },
 "nbformat": 4,
 "nbformat_minor": 4
}
